fixed the issue in the CIVL version of treiber stack

treiber-stack/desugared.out.bpl
@@ -1,80 +1,78 @@
 // Boogie program verifier version 3.0.5.0, Copyright (c) 2003-2014, Microsoft.
 // Command Line Options: -trace -lib:base -lib:node -civlDesugaredFile:desugared.out.bpl treiber-stack-linked-list.bpl
 
-type Heap = PolymorphicMapType_5905;
+type Heap = PolymorphicMapType_5887;
 
-var heap: PolymorphicMapType_5905;
+var heap: PolymorphicMapType_5887;
 
-var head: Ref_5929;
+var head: Ref_5911;
 
 const Identity: [int]int;
 
 function {:inline} AtLeast(x: int) : [int]bool
 {
-  MapLe_1179(MapConst_1196_1179(x), Identity)
+  MapLe_1169(MapConst_1186_1169(x), Identity)
 }
 
 function {:inline} Range(from: int, n: int) : [int]bool
 {
-  MapDiff_1199(AtLeast(from), AtLeast(from + n))
+  MapDiff_1189(AtLeast(from), AtLeast(from + n))
 }
 
 type {:builtin "Seq"} Seq _;
 
 datatype Node_31 {
-  Node_31(next: Ref_5929, val: int)
+  Node_31(next: Ref_5911, val: int)
 }
 
-type Ref_5929;
+type Ref_5911;
 
-datatype Option_5952 {
-  None_5952(),
-  Some_5952(t: Node_31)
+datatype Option_5934 {
+  None_5934(),
+  Some_5934(t: Node_31)
 }
 
-datatype Lval_7085 {
-  Lval_7085(val: Ref_5929)
+datatype Lval_6847 {
+  Lval_6847(val: Ref_5911)
 }
 
-procedure Ref_Alloc_7109() returns (k: Lval_7085);
+procedure Ref_Alloc_6871() returns (k: Lval_6847);
 
 
 
-function {:builtin "MapConst"} MapConst_1196_1179(int) : [int]int;
+function {:builtin "MapConst"} MapConst_1186_1169(int) : [int]int;
 
-function {:builtin "MapLe"} MapLe_1179([int]int, [int]int) : [int]bool;
+function {:builtin "MapLe"} MapLe_1169([int]int, [int]int) : [int]bool;
 
-function {:inline} MapDiff_1199(a: [int]bool, b: [int]bool) : [int]bool
+function {:inline} MapDiff_1189(a: [int]bool, b: [int]bool) : [int]bool
 {
-  MapAnd_1199(a, MapNot_1199(b))
+  MapAnd_1189(a, MapNot_1189(b))
 }
 
-function {:builtin "MapNot"} MapNot_1199([int]bool) : [int]bool;
+function {:builtin "MapNot"} MapNot_1189([int]bool) : [int]bool;
 
-function {:builtin "MapAnd"} MapAnd_1199([int]bool, [int]bool) : [int]bool;
+function {:builtin "MapAnd"} MapAnd_1189([int]bool, [int]bool) : [int]bool;
 
-datatype Vec_1196 {
-  Vec_1196(contents: [int]int, len: int)
+datatype Vec_1186 {
+  Vec_1186(contents: [int]int, len: int)
 }
 
-function Default_1196() : int;
+function Default_1186() : int;
 
-function {:builtin "MapIte"} MapIte_1220_1196([int]bool, [int]int, [int]int) : [int]int;
+function {:builtin "MapIte"} MapIte_1210_1186([int]bool, [int]int, [int]int) : [int]int;
 
-function Between_31(f: [Ref_5929]Node_31, x: Ref_5929, y: Ref_5929, z: Ref_5929) : bool;
+function Between_31(f: [Ref_5911]Node_31, x: Ref_5911, y: Ref_5911, z: Ref_5911) : bool;
 
-function Avoiding_31(f: [Ref_5929]Node_31, x: Ref_5929, y: Ref_5929, z: Ref_5929) : bool;
+function Avoiding_31(f: [Ref_5911]Node_31, x: Ref_5911, y: Ref_5911, z: Ref_5911) : bool;
 
 axiom (forall x: int :: Identity[x] == x);
 
-axiom (forall x: Vec_1196 :: 
+axiom (forall x: Vec_1186 :: 
   { x->len } { x->contents } 
-  MapIte_1220_1196(Range(0, x->len), MapConst_1196_1179(Default_1196()), x->contents)
-     == MapConst_1196_1179(Default_1196()));
+  MapIte_1210_1186(Range(0, x->len), MapConst_1186_1169(Default_1186()), x->contents)
+     == MapConst_1186_1169(Default_1186()));
 
-axiom (forall x: Vec_1196 :: { x->len } x->len >= 0);
-
-axiom true;
+axiom (forall x: Vec_1186 :: { x->len } x->len >= 0);
 
 axiom true;
 
@@ -88,65 +86,67 @@ axiom true;
 
 axiom true;
 
-axiom (forall f: [Ref_5929]Node_31, x: Ref_5929 :: Between_31(f, x, x, x));
+axiom true;
 
-axiom (forall f: [Ref_5929]Node_31, x: Ref_5929, y: Ref_5929, z: Ref_5929, w: Ref_5929 :: 
+axiom (forall f: [Ref_5911]Node_31, x: Ref_5911 :: Between_31(f, x, x, x));
+
+axiom (forall f: [Ref_5911]Node_31, x: Ref_5911, y: Ref_5911, z: Ref_5911, w: Ref_5911 :: 
   { Between_31(f, y, z, w), f[x] } 
   Between_31(f, x, f[x]->next, f[x]->next));
 
-axiom (forall f: [Ref_5929]Node_31, x: Ref_5929, y: Ref_5929 :: 
+axiom (forall f: [Ref_5911]Node_31, x: Ref_5911, y: Ref_5911 :: 
   { f[x], Between_31(f, x, y, y) } 
   Between_31(f, x, y, y) ==> x == y || Between_31(f, x, f[x]->next, y));
 
-axiom (forall f: [Ref_5929]Node_31, x: Ref_5929, y: Ref_5929 :: 
+axiom (forall f: [Ref_5911]Node_31, x: Ref_5911, y: Ref_5911 :: 
   { f[x], Between_31(f, x, y, y) } 
   f[x]->next == x && Between_31(f, x, y, y) ==> x == y);
 
-axiom (forall f: [Ref_5929]Node_31, x: Ref_5929, y: Ref_5929 :: 
+axiom (forall f: [Ref_5911]Node_31, x: Ref_5911, y: Ref_5911 :: 
   { Between_31(f, x, y, x) } 
   Between_31(f, x, y, x) ==> x == y);
 
-axiom (forall f: [Ref_5929]Node_31, x: Ref_5929, y: Ref_5929, z: Ref_5929 :: 
+axiom (forall f: [Ref_5911]Node_31, x: Ref_5911, y: Ref_5911, z: Ref_5911 :: 
   { Between_31(f, x, y, y), Between_31(f, x, z, z) } 
   Between_31(f, x, y, y) && Between_31(f, x, z, z)
      ==> Between_31(f, x, y, z) || Between_31(f, x, z, y));
 
-axiom (forall f: [Ref_5929]Node_31, x: Ref_5929, y: Ref_5929, z: Ref_5929 :: 
+axiom (forall f: [Ref_5911]Node_31, x: Ref_5911, y: Ref_5911, z: Ref_5911 :: 
   { Between_31(f, x, y, z) } 
   Between_31(f, x, y, z) ==> Between_31(f, x, y, y) && Between_31(f, y, z, z));
 
-axiom (forall f: [Ref_5929]Node_31, x: Ref_5929, y: Ref_5929, z: Ref_5929 :: 
+axiom (forall f: [Ref_5911]Node_31, x: Ref_5911, y: Ref_5911, z: Ref_5911 :: 
   { Between_31(f, x, y, y), Between_31(f, y, z, z) } 
   Between_31(f, x, y, y) && Between_31(f, y, z, z) ==> Between_31(f, x, z, z));
 
-axiom (forall f: [Ref_5929]Node_31, x: Ref_5929, y: Ref_5929, z: Ref_5929, w: Ref_5929 :: 
+axiom (forall f: [Ref_5911]Node_31, x: Ref_5911, y: Ref_5911, z: Ref_5911, w: Ref_5911 :: 
   { Between_31(f, x, y, z), Between_31(f, y, w, z) } 
   Between_31(f, x, y, z) && Between_31(f, y, w, z)
      ==> Between_31(f, x, y, w) && Between_31(f, x, w, z));
 
-axiom (forall f: [Ref_5929]Node_31, x: Ref_5929, y: Ref_5929, z: Ref_5929, w: Ref_5929 :: 
+axiom (forall f: [Ref_5911]Node_31, x: Ref_5911, y: Ref_5911, z: Ref_5911, w: Ref_5911 :: 
   { Between_31(f, x, y, z), Between_31(f, x, w, y) } 
   Between_31(f, x, y, z) && Between_31(f, x, w, y)
      ==> Between_31(f, x, w, z) && Between_31(f, w, y, z));
 
-axiom (forall f: [Ref_5929]Node_31, u: Ref_5929, x: Ref_5929 :: 
+axiom (forall f: [Ref_5911]Node_31, u: Ref_5911, x: Ref_5911 :: 
   { Between_31(f, u, x, x) } 
   Between_31(f, u, x, x) ==> Between_31(f, u, u, x));
 
-axiom (forall f: [Ref_5929]Node_31, x: Ref_5929, y: Ref_5929, z: Ref_5929 :: 
+axiom (forall f: [Ref_5911]Node_31, x: Ref_5911, y: Ref_5911, z: Ref_5911 :: 
   { Avoiding_31(f, x, y, z) } 
   Avoiding_31(f, x, y, z)
      <==> Between_31(f, x, y, z) || (Between_31(f, x, y, y) && !Between_31(f, x, z, z)));
 
-axiom (forall f: [Ref_5929]Node_31, x: Ref_5929, y: Ref_5929, z: Ref_5929 :: 
+axiom (forall f: [Ref_5911]Node_31, x: Ref_5911, y: Ref_5911, z: Ref_5911 :: 
   { Between_31(f, x, y, z) } 
   Between_31(f, x, y, z) <==> Avoiding_31(f, x, y, z) && Avoiding_31(f, x, z, z));
 
-axiom (forall f: [Ref_5929]Node_31, 
-    u: Ref_5929, 
-    v: Ref_5929, 
-    x: Ref_5929, 
-    p: Ref_5929, 
+axiom (forall f: [Ref_5911]Node_31, 
+    u: Ref_5911, 
+    v: Ref_5911, 
+    x: Ref_5911, 
+    p: Ref_5911, 
     q: Node_31 :: 
   { Avoiding_31(f[p := q], u, v, x) } 
   Avoiding_31(f[p := q], u, v, x)
@@ -157,50 +157,60 @@ axiom (forall f: [Ref_5929]Node_31,
          && Avoiding_31(f, q->next, v, p)
          && Avoiding_31(f, q->next, v, x)));
 
-datatype PolymorphicMapType_5905 {
-  PolymorphicMapType_5905(PolymorphicMapType_5905_38: [Ref_5929]Option_5952)
+datatype PolymorphicMapType_5887 {
+  PolymorphicMapType_5887(PolymorphicMapType_5887_38: [Ref_5911]Option_5934)
 }
 
-function {:inline} Lval_Collector_7085(l: Lval_7085) : [Ref_5929]bool
+function {:inline} Lval_Collector_6847(l: Lval_6847) : [Ref_5911]bool
 {
-  MapConst_5_7085(false)[l->val := true]
+  MapConst_5_6847(false)[l->val := true]
 }
 
-function {:builtin "MapConst"} MapConst_5_7085(bool) : [Ref_5929]bool;
+function {:builtin "MapConst"} MapConst_5_6847(bool) : [Ref_5911]bool;
 
-function {:builtin "MapConst"} MapConst_3_7085(int) : [Ref_5929]int;
+function {:builtin "MapConst"} MapConst_3_6847(int) : [Ref_5911]int;
 
-function {:builtin "MapOr"} MapOr_7085([Ref_5929]bool, [Ref_5929]bool) : [Ref_5929]bool;
+function {:builtin "MapOr"} MapOr_6847([Ref_5911]bool, [Ref_5911]bool) : [Ref_5911]bool;
 
-function {:builtin "MapImp"} MapImp_7085([Ref_5929]bool, [Ref_5929]bool) : [Ref_5929]bool;
+function {:builtin "MapImp"} MapImp_6847([Ref_5911]bool, [Ref_5911]bool) : [Ref_5911]bool;
 
-function {:builtin "MapEq"} MapEq_7085_3([Ref_5929]int, [Ref_5929]int) : [Ref_5929]bool;
+function {:builtin "MapEq"} MapEq_6847_3([Ref_5911]int, [Ref_5911]int) : [Ref_5911]bool;
 
-function {:builtin "MapAdd"} MapAdd_7085([Ref_5929]int, [Ref_5929]int) : [Ref_5929]int;
+function {:builtin "MapAdd"} MapAdd_6847([Ref_5911]int, [Ref_5911]int) : [Ref_5911]int;
 
-function {:builtin "MapIte"} MapIte_7085_3([Ref_5929]bool, [Ref_5929]int, [Ref_5929]int) : [Ref_5929]int;
+function {:builtin "MapIte"} MapIte_6847_3([Ref_5911]bool, [Ref_5911]int, [Ref_5911]int) : [Ref_5911]int;
 
-function {:builtin "MapLe"} MapLe_7085([Ref_5929]int, [Ref_5929]int) : [Ref_5929]bool;
+function {:builtin "MapLe"} MapLe_6847([Ref_5911]int, [Ref_5911]int) : [Ref_5911]bool;
 
-datatype Lheap_7109 {
-  Lheap_7109(dom: [Ref_5929]bool, val: [Ref_5929]Node_31)
+datatype Lheap_6871 {
+  Lheap_6871(dom: [Ref_5911]bool, val: [Ref_5911]Node_31)
 }
 
-datatype Lset_7109 {
-  Lset_7109(dom: [Node_31]bool)
+datatype Lset_6871 {
+  Lset_6871(dom: [Node_31]bool)
 }
 
-datatype Lval_7109 {
-  Lval_7109(val: Node_31)
+datatype Lval_6871 {
+  Lval_6871(val: Node_31)
 }
 
-function Nil_7109() : Ref_5929;
+function Nil_6871() : Ref_5911;
 
-function Trigger_SpecSetRefVal__heap(_heap: PolymorphicMapType_5905) : bool;
+function Trigger_SpecSetRefVal__heap(_heap: PolymorphicMapType_5887) : bool;
 
-function Trigger_SpecGetRefVal__heap(_heap: PolymorphicMapType_5905) : bool;
+function Trigger_SpecGetRefVal__heap(_heap: PolymorphicMapType_5887) : bool;
 
 function Trigger_SpecCAS_Head_eq(eq: bool) : bool;
+
+function Trigger_SpecCAS_Head_headNode(headNode: Node_31) : bool;
+
+function Trigger_SpecCAS_Head_inline$SpecGetRefVal$0$_heap(inline$SpecGetRefVal$0$_heap: PolymorphicMapType_5887) : bool;
+
+function Trigger_SpecCAS_Head_inline$SpecGetRefVal$0$ref(inline$SpecGetRefVal$0$ref: Ref_5911) : bool;
+
+function Trigger_SpecCAS_Head_inline$SpecGetRefVal$0$x(inline$SpecGetRefVal$0$x: Node_31) : bool;
+
+function Trigger_SpecCAS_Head_inline$SpecGetRefVal$0$heap(inline$SpecGetRefVal$0$heap: PolymorphicMapType_5887) : bool;
 
 function Trigger_SpecCAS_Head_inline$SpecNodeEq$0$n1(inline$SpecNodeEq$0$n1: Node_31) : bool;
 
@@ -208,114 +218,142 @@ function Trigger_SpecCAS_Head_inline$SpecNodeEq$0$n2(inline$SpecNodeEq$0$n2: Nod
 
 function Trigger_SpecCAS_Head_inline$SpecNodeEq$0$eq(inline$SpecNodeEq$0$eq: bool) : bool;
 
-function Trigger_SpecCAS_Head_inline$SpecSetRefVal$0$_heap(inline$SpecSetRefVal$0$_heap: PolymorphicMapType_5905) : bool;
+function Trigger_SpecCAS_Head_inline$SpecSetRefVal$0$_heap(inline$SpecSetRefVal$0$_heap: PolymorphicMapType_5887) : bool;
 
-function Trigger_SpecCAS_Head_inline$SpecSetRefVal$0$ref(inline$SpecSetRefVal$0$ref: Ref_5929) : bool;
+function Trigger_SpecCAS_Head_inline$SpecSetRefVal$0$ref(inline$SpecSetRefVal$0$ref: Ref_5911) : bool;
 
-function Trigger_SpecCAS_Head_inline$SpecSetRefVal$0$x(inline$SpecSetRefVal$0$x: Option_5952) : bool;
+function Trigger_SpecCAS_Head_inline$SpecSetRefVal$0$x(inline$SpecSetRefVal$0$x: Option_5934) : bool;
 
-function Trigger_SpecCAS_Head_inline$SpecSetRefVal$0$heap(inline$SpecSetRefVal$0$heap: PolymorphicMapType_5905) : bool;
+function Trigger_SpecCAS_Head_inline$SpecSetRefVal$0$heap(inline$SpecSetRefVal$0$heap: PolymorphicMapType_5887) : bool;
 
-function Trigger_SpecAllocNodeRef_inline$SpecSetRefVal$0$_heap(inline$SpecSetRefVal$0$_heap: PolymorphicMapType_5905) : bool;
+function Trigger_SpecAllocNodeRef_inline$SpecSetRefVal$0$_heap(inline$SpecSetRefVal$0$_heap: PolymorphicMapType_5887) : bool;
 
-function Trigger_SpecAllocNodeRef_inline$SpecSetRefVal$0$ref(inline$SpecSetRefVal$0$ref: Ref_5929) : bool;
+function Trigger_SpecAllocNodeRef_inline$SpecSetRefVal$0$ref(inline$SpecSetRefVal$0$ref: Ref_5911) : bool;
 
-function Trigger_SpecAllocNodeRef_inline$SpecSetRefVal$0$x(inline$SpecSetRefVal$0$x: Option_5952) : bool;
+function Trigger_SpecAllocNodeRef_inline$SpecSetRefVal$0$x(inline$SpecSetRefVal$0$x: Option_5934) : bool;
 
-function Trigger_SpecAllocNodeRef_inline$SpecSetRefVal$0$heap(inline$SpecSetRefVal$0$heap: PolymorphicMapType_5905) : bool;
+function Trigger_SpecAllocNodeRef_inline$SpecSetRefVal$0$heap(inline$SpecSetRefVal$0$heap: PolymorphicMapType_5887) : bool;
 
-function Trigger_SpecPush_newHeadRef(newHeadRef: Lval_7085) : bool;
+function Trigger_SpecPop_oldHead(oldHead: Node_31) : bool;
+
+function Trigger_SpecPop_newHead(newHead: Node_31) : bool;
+
+function Trigger_SpecPop_inline$SpecGetRefVal$0$_heap(inline$SpecGetRefVal$0$_heap: PolymorphicMapType_5887) : bool;
+
+function Trigger_SpecPop_inline$SpecGetRefVal$0$ref(inline$SpecGetRefVal$0$ref: Ref_5911) : bool;
+
+function Trigger_SpecPop_inline$SpecGetRefVal$0$x(inline$SpecGetRefVal$0$x: Node_31) : bool;
+
+function Trigger_SpecPop_inline$SpecGetRefVal$0$heap(inline$SpecGetRefVal$0$heap: PolymorphicMapType_5887) : bool;
+
+function Trigger_SpecPop_inline$SpecGetRefVal$1$_heap(inline$SpecGetRefVal$1$_heap: PolymorphicMapType_5887) : bool;
+
+function Trigger_SpecPop_inline$SpecGetRefVal$1$ref(inline$SpecGetRefVal$1$ref: Ref_5911) : bool;
+
+function Trigger_SpecPop_inline$SpecGetRefVal$1$x(inline$SpecGetRefVal$1$x: Node_31) : bool;
+
+function Trigger_SpecPop_inline$SpecGetRefVal$1$heap(inline$SpecGetRefVal$1$heap: PolymorphicMapType_5887) : bool;
+
+function Trigger_SpecPop_inline$SpecSetRefVal$0$_heap(inline$SpecSetRefVal$0$_heap: PolymorphicMapType_5887) : bool;
+
+function Trigger_SpecPop_inline$SpecSetRefVal$0$ref(inline$SpecSetRefVal$0$ref: Ref_5911) : bool;
+
+function Trigger_SpecPop_inline$SpecSetRefVal$0$x(inline$SpecSetRefVal$0$x: Option_5934) : bool;
+
+function Trigger_SpecPop_inline$SpecSetRefVal$0$heap(inline$SpecSetRefVal$0$heap: PolymorphicMapType_5887) : bool;
+
+function Trigger_SpecPush_newHeadRef(newHeadRef: Lval_6847) : bool;
 
 function Trigger_SpecPush_newHead(newHead: Node_31) : bool;
 
-function Trigger_SpecPush_inline$SpecAllocNodeRef$0$k(inline$SpecAllocNodeRef$0$k: Lval_7085) : bool;
+function Trigger_SpecPush_inline$SpecAllocNodeRef$0$k(inline$SpecAllocNodeRef$0$k: Lval_6847) : bool;
 
-function Trigger_SpecPush_inline$SpecAllocNodeRef$0$heap(inline$SpecAllocNodeRef$0$heap: PolymorphicMapType_5905) : bool;
+function Trigger_SpecPush_inline$SpecAllocNodeRef$0$heap(inline$SpecAllocNodeRef$0$heap: PolymorphicMapType_5887) : bool;
 
-function Trigger_SpecPush_inline$SpecSetRefVal$0$_heap(inline$SpecSetRefVal$0$_heap: PolymorphicMapType_5905) : bool;
+function Trigger_SpecPush_inline$SpecSetRefVal$0$_heap(inline$SpecSetRefVal$0$_heap: PolymorphicMapType_5887) : bool;
 
-function Trigger_SpecPush_inline$SpecSetRefVal$0$ref(inline$SpecSetRefVal$0$ref: Ref_5929) : bool;
+function Trigger_SpecPush_inline$SpecSetRefVal$0$ref(inline$SpecSetRefVal$0$ref: Ref_5911) : bool;
 
-function Trigger_SpecPush_inline$SpecSetRefVal$0$x(inline$SpecSetRefVal$0$x: Option_5952) : bool;
+function Trigger_SpecPush_inline$SpecSetRefVal$0$x(inline$SpecSetRefVal$0$x: Option_5934) : bool;
 
-function Trigger_SpecPush_inline$SpecSetRefVal$0$heap(inline$SpecSetRefVal$0$heap: PolymorphicMapType_5905) : bool;
+function Trigger_SpecPush_inline$SpecSetRefVal$0$heap(inline$SpecSetRefVal$0$heap: PolymorphicMapType_5887) : bool;
 
-function Trigger_SpecPush_inline$SpecGetRefVal$0$_heap(inline$SpecGetRefVal$0$_heap: PolymorphicMapType_5905) : bool;
+function Trigger_SpecPush_inline$SpecGetRefVal$0$_heap(inline$SpecGetRefVal$0$_heap: PolymorphicMapType_5887) : bool;
 
-function Trigger_SpecPush_inline$SpecGetRefVal$0$ref(inline$SpecGetRefVal$0$ref: Ref_5929) : bool;
+function Trigger_SpecPush_inline$SpecGetRefVal$0$ref(inline$SpecGetRefVal$0$ref: Ref_5911) : bool;
 
 function Trigger_SpecPush_inline$SpecGetRefVal$0$x(inline$SpecGetRefVal$0$x: Node_31) : bool;
 
-function Trigger_SpecPush_inline$SpecGetRefVal$0$heap(inline$SpecGetRefVal$0$heap: PolymorphicMapType_5905) : bool;
+function Trigger_SpecPush_inline$SpecGetRefVal$0$heap(inline$SpecGetRefVal$0$heap: PolymorphicMapType_5887) : bool;
 
-function Trigger_SpecPush_inline$SpecSetRefVal$1$_heap(inline$SpecSetRefVal$1$_heap: PolymorphicMapType_5905) : bool;
+function Trigger_SpecPush_inline$SpecSetRefVal$1$_heap(inline$SpecSetRefVal$1$_heap: PolymorphicMapType_5887) : bool;
 
-function Trigger_SpecPush_inline$SpecSetRefVal$1$ref(inline$SpecSetRefVal$1$ref: Ref_5929) : bool;
+function Trigger_SpecPush_inline$SpecSetRefVal$1$ref(inline$SpecSetRefVal$1$ref: Ref_5911) : bool;
 
-function Trigger_SpecPush_inline$SpecSetRefVal$1$x(inline$SpecSetRefVal$1$x: Option_5952) : bool;
+function Trigger_SpecPush_inline$SpecSetRefVal$1$x(inline$SpecSetRefVal$1$x: Option_5934) : bool;
 
-function Trigger_SpecPush_inline$SpecSetRefVal$1$heap(inline$SpecSetRefVal$1$heap: PolymorphicMapType_5905) : bool;
+function Trigger_SpecPush_inline$SpecSetRefVal$1$heap(inline$SpecSetRefVal$1$heap: PolymorphicMapType_5887) : bool;
 
-implementation SpecSetRefVal(ref: Ref_5929, x: Option_5952)
+implementation SpecSetRefVal(ref: Ref_5911, x: Option_5934)
 {
-  var _heap: PolymorphicMapType_5905;
+  var _heap: PolymorphicMapType_5887;
 
   /*** structured program:
     _heap := old(heap);
-    _heap->PolymorphicMapType_5905_38[ref] := x;
+    _heap->PolymorphicMapType_5887_38[ref] := x;
   **** end structured program */
 
   anon0:
     _heap := old(heap);
-    _heap->PolymorphicMapType_5905_38[ref] := x;
+    _heap->PolymorphicMapType_5887_38[ref] := x;
     return;
 }
 
 
 
-procedure {:inline 1} SpecSetRefVal(ref: Ref_5929, x: Option_5952);
+procedure {:inline 1} SpecSetRefVal(ref: Ref_5911, x: Option_5934);
   modifies heap;
 
 
 
-function {:inline} Civl_InputOutputRelation_SpecSetRefVal(ref: Ref_5929, x: Option_5952) : bool
+function {:inline} Civl_InputOutputRelation_SpecSetRefVal(ref: Ref_5911, x: Option_5934) : bool
 {
-  (exists Civl_old_heap: PolymorphicMapType_5905, 
-      Civl_old_head: Ref_5929, 
-      Civl_heap: PolymorphicMapType_5905, 
-      Civl_head: Ref_5929 :: 
+  (exists Civl_old_heap: PolymorphicMapType_5887, 
+      Civl_old_head: Ref_5911, 
+      Civl_heap: PolymorphicMapType_5887, 
+      Civl_head: Ref_5911 :: 
     Civl_heap == Civl_old_heap)
 }
 
-implementation SpecGetRefVal(ref: Ref_5929) returns (x: Node_31)
+implementation SpecGetRefVal(ref: Ref_5911) returns (x: Node_31)
 {
-  var _heap: PolymorphicMapType_5905;
+  var _heap: PolymorphicMapType_5887;
 
   /*** structured program:
     _heap := old(heap);
-    x := _heap->PolymorphicMapType_5905_38[ref]->t;
+    x := _heap->PolymorphicMapType_5887_38[ref]->t;
   **** end structured program */
 
   anon0:
     _heap := old(heap);
-    x := _heap->PolymorphicMapType_5905_38[ref]->t;
+    x := _heap->PolymorphicMapType_5887_38[ref]->t;
     return;
 }
 
 
 
-procedure {:inline 1} SpecGetRefVal(ref: Ref_5929) returns (x: Node_31);
+procedure {:inline 1} SpecGetRefVal(ref: Ref_5911) returns (x: Node_31);
   modifies heap;
 
 
 
-function {:inline} Civl_InputOutputRelation_SpecGetRefVal(ref: Ref_5929, x: Node_31) : bool
+function {:inline} Civl_InputOutputRelation_SpecGetRefVal(ref: Ref_5911, x: Node_31) : bool
 {
-  (exists Civl_old_heap: PolymorphicMapType_5905, 
-      Civl_old_head: Ref_5929, 
-      Civl_heap: PolymorphicMapType_5905, 
-      Civl_head: Ref_5929 :: 
-    x == Civl_heap->PolymorphicMapType_5905_38[ref]->t && Civl_heap == Civl_old_heap)
+  (exists Civl_old_heap: PolymorphicMapType_5887, 
+      Civl_old_head: Ref_5911, 
+      Civl_heap: PolymorphicMapType_5887, 
+      Civl_head: Ref_5911 :: 
+    x == Civl_heap->PolymorphicMapType_5887_38[ref]->t && Civl_heap == Civl_old_heap)
 }
 
 implementation SpecNodeEq(n1: Node_31, n2: Node_31) returns (eq: bool)
@@ -337,37 +375,66 @@ procedure {:inline 1} SpecNodeEq(n1: Node_31, n2: Node_31) returns (eq: bool);
 
 function {:inline} Civl_InputOutputRelation_SpecNodeEq(n1: Node_31, n2: Node_31, eq: bool) : bool
 {
-  (exists Civl_old_heap: PolymorphicMapType_5905, 
-      Civl_old_head: Ref_5929, 
-      Civl_heap: PolymorphicMapType_5905, 
-      Civl_head: Ref_5929 :: 
+  (exists Civl_old_heap: PolymorphicMapType_5887, 
+      Civl_old_head: Ref_5911, 
+      Civl_heap: PolymorphicMapType_5887, 
+      Civl_head: Ref_5911 :: 
     eq <==> n1 == n2)
 }
 
 implementation SpecCAS_Head(expectedNode: Node_31, desiredNode: Node_31) returns (success: bool)
 {
   var eq: bool;
+  var headNode: Node_31;
+  var inline$SpecGetRefVal$0$_heap: PolymorphicMapType_5887;
+  var inline$SpecGetRefVal$0$ref: Ref_5911;
+  var inline$SpecGetRefVal$0$x: Node_31;
+  var inline$SpecGetRefVal$0$heap: PolymorphicMapType_5887;
   var inline$SpecNodeEq$0$n1: Node_31;
   var inline$SpecNodeEq$0$n2: Node_31;
   var inline$SpecNodeEq$0$eq: bool;
-  var inline$SpecSetRefVal$0$_heap: PolymorphicMapType_5905;
-  var inline$SpecSetRefVal$0$ref: Ref_5929;
-  var inline$SpecSetRefVal$0$x: Option_5952;
-  var inline$SpecSetRefVal$0$heap: PolymorphicMapType_5905;
+  var inline$SpecSetRefVal$0$_heap: PolymorphicMapType_5887;
+  var inline$SpecSetRefVal$0$ref: Ref_5911;
+  var inline$SpecSetRefVal$0$x: Option_5934;
+  var inline$SpecSetRefVal$0$heap: PolymorphicMapType_5887;
 
   /*** structured program:
-    call eq := SpecNodeEq(heap->PolymorphicMapType_5905_38[head]->t, expectedNode);
+    call headNode := SpecGetRefVal(head);
+    call eq := SpecNodeEq(headNode, expectedNode);
     if (eq)
     {
-        call SpecSetRefVal(head, Some_5952(desiredNode));
+        call SpecSetRefVal(head, Some_5934(desiredNode));
+        success := true;
+    }
+    else
+    {
+        success := false;
     }
   **** end structured program */
 
   anon0:
+    goto inline$SpecGetRefVal$0$Entry;
+
+  inline$SpecGetRefVal$0$Entry:
+    inline$SpecGetRefVal$0$ref := head;
+    havoc inline$SpecGetRefVal$0$_heap, inline$SpecGetRefVal$0$x;
+    inline$SpecGetRefVal$0$heap := heap;
+    goto inline$SpecGetRefVal$0$anon0;
+
+  inline$SpecGetRefVal$0$anon0:
+    inline$SpecGetRefVal$0$_heap := inline$SpecGetRefVal$0$heap;
+    inline$SpecGetRefVal$0$x := inline$SpecGetRefVal$0$_heap->PolymorphicMapType_5887_38[inline$SpecGetRefVal$0$ref]->t;
+    goto inline$SpecGetRefVal$0$Return;
+
+  inline$SpecGetRefVal$0$Return:
+    headNode := inline$SpecGetRefVal$0$x;
+    goto anon0$1;
+
+  anon0$1:
     goto inline$SpecNodeEq$0$Entry;
 
   inline$SpecNodeEq$0$Entry:
-    inline$SpecNodeEq$0$n1 := heap->PolymorphicMapType_5905_38[head]->t;
+    inline$SpecNodeEq$0$n1 := headNode;
     inline$SpecNodeEq$0$n2 := expectedNode;
     havoc inline$SpecNodeEq$0$eq;
     goto inline$SpecNodeEq$0$anon0;
@@ -378,35 +445,37 @@ implementation SpecCAS_Head(expectedNode: Node_31, desiredNode: Node_31) returns
 
   inline$SpecNodeEq$0$Return:
     eq := inline$SpecNodeEq$0$eq;
-    goto anon0$1;
+    goto anon0$2;
 
-  anon0$1:
-    goto anon2_Then, anon2_Else;
+  anon0$2:
+    goto anon3_Then, anon3_Else;
 
-  anon2_Else:
+  anon3_Else:
     assume {:partition} !eq;
+    success := false;
     return;
 
-  anon2_Then:
+  anon3_Then:
     assume {:partition} eq;
     goto inline$SpecSetRefVal$0$Entry;
 
   inline$SpecSetRefVal$0$Entry:
     inline$SpecSetRefVal$0$ref := head;
-    inline$SpecSetRefVal$0$x := Some_5952(desiredNode);
+    inline$SpecSetRefVal$0$x := Some_5934(desiredNode);
     havoc inline$SpecSetRefVal$0$_heap;
     inline$SpecSetRefVal$0$heap := heap;
     goto inline$SpecSetRefVal$0$anon0;
 
   inline$SpecSetRefVal$0$anon0:
     inline$SpecSetRefVal$0$_heap := inline$SpecSetRefVal$0$heap;
-    inline$SpecSetRefVal$0$_heap->PolymorphicMapType_5905_38[inline$SpecSetRefVal$0$ref] := inline$SpecSetRefVal$0$x;
+    inline$SpecSetRefVal$0$_heap->PolymorphicMapType_5887_38[inline$SpecSetRefVal$0$ref] := inline$SpecSetRefVal$0$x;
     goto inline$SpecSetRefVal$0$Return;
 
   inline$SpecSetRefVal$0$Return:
-    goto anon2_Then$1;
+    goto anon3_Then$1;
 
-  anon2_Then$1:
+  anon3_Then$1:
+    success := true;
     return;
 }
 
@@ -419,43 +488,47 @@ procedure {:inline 1} SpecCAS_Head(expectedNode: Node_31, desiredNode: Node_31) 
 
 function {:inline} Civl_InputOutputRelation_SpecCAS_Head(expectedNode: Node_31, desiredNode: Node_31, success: bool) : bool
 {
-  (exists Civl_old_heap: PolymorphicMapType_5905, 
-      Civl_old_head: Ref_5929, 
-      Civl_heap: PolymorphicMapType_5905, 
-      Civl_head: Ref_5929 :: 
-    (Civl_heap->PolymorphicMapType_5905_38[Civl_head]->t == expectedNode
+  (exists Civl_old_heap: PolymorphicMapType_5887, 
+      Civl_old_head: Ref_5911, 
+      Civl_heap: PolymorphicMapType_5887, 
+      Civl_head: Ref_5911 :: 
+    (
+        Civl_heap->PolymorphicMapType_5887_38[Civl_head]->t == expectedNode
+         && (success <==> true)
          && Civl_heap == Civl_old_heap)
-       || (!(Civl_heap->PolymorphicMapType_5905_38[Civl_head]->t == expectedNode)
+       || (
+        !(Civl_heap->PolymorphicMapType_5887_38[Civl_head]->t == expectedNode)
+         && (success <==> false)
          && Civl_heap == Civl_old_heap))
 }
 
-implementation SpecAllocNodeRef() returns (k: Lval_7085)
+implementation SpecAllocNodeRef() returns (k: Lval_6847)
 {
-  var inline$SpecSetRefVal$0$_heap: PolymorphicMapType_5905;
-  var inline$SpecSetRefVal$0$ref: Ref_5929;
-  var inline$SpecSetRefVal$0$x: Option_5952;
-  var inline$SpecSetRefVal$0$heap: PolymorphicMapType_5905;
+  var inline$SpecSetRefVal$0$_heap: PolymorphicMapType_5887;
+  var inline$SpecSetRefVal$0$ref: Ref_5911;
+  var inline$SpecSetRefVal$0$x: Option_5934;
+  var inline$SpecSetRefVal$0$heap: PolymorphicMapType_5887;
 
   /*** structured program:
-    call k := Ref_Alloc_7109();
-    call SpecSetRefVal(k->val, None_5952());
+    call k := Ref_Alloc_6871();
+    call SpecSetRefVal(k->val, None_5934());
   **** end structured program */
 
   anon0:
     havoc k;
-    assume k->val != Nil_7109();
+    assume k->val != Nil_6871();
     goto inline$SpecSetRefVal$0$Entry;
 
   inline$SpecSetRefVal$0$Entry:
     inline$SpecSetRefVal$0$ref := k->val;
-    inline$SpecSetRefVal$0$x := None_5952();
+    inline$SpecSetRefVal$0$x := None_5934();
     havoc inline$SpecSetRefVal$0$_heap;
     inline$SpecSetRefVal$0$heap := heap;
     goto inline$SpecSetRefVal$0$anon0;
 
   inline$SpecSetRefVal$0$anon0:
     inline$SpecSetRefVal$0$_heap := inline$SpecSetRefVal$0$heap;
-    inline$SpecSetRefVal$0$_heap->PolymorphicMapType_5905_38[inline$SpecSetRefVal$0$ref] := inline$SpecSetRefVal$0$x;
+    inline$SpecSetRefVal$0$_heap->PolymorphicMapType_5887_38[inline$SpecSetRefVal$0$ref] := inline$SpecSetRefVal$0$x;
     goto inline$SpecSetRefVal$0$Return;
 
   inline$SpecSetRefVal$0$Return:
@@ -467,45 +540,146 @@ implementation SpecAllocNodeRef() returns (k: Lval_7085)
 
 
 
-procedure {:inline 1} SpecAllocNodeRef() returns (k: Lval_7085);
+procedure {:inline 1} SpecAllocNodeRef() returns (k: Lval_6847);
   modifies heap;
 
 
 
-function {:inline} Civl_InputOutputRelation_SpecAllocNodeRef(k: Lval_7085) : bool
+function {:inline} Civl_InputOutputRelation_SpecAllocNodeRef(k: Lval_6847) : bool
 {
-  (exists Civl_old_heap: PolymorphicMapType_5905, 
-      Civl_old_head: Ref_5929, 
-      Civl_heap: PolymorphicMapType_5905, 
-      Civl_head: Ref_5929 :: 
-    k->val != Nil_7109() && Civl_heap == Civl_old_heap)
+  (exists Civl_old_heap: PolymorphicMapType_5887, 
+      Civl_old_head: Ref_5911, 
+      Civl_heap: PolymorphicMapType_5887, 
+      Civl_head: Ref_5911 :: 
+    k->val != Nil_6871() && Civl_heap == Civl_old_heap)
+}
+
+implementation SpecPop() returns (item: int)
+{
+  var oldHead: Node_31;
+  var newHead: Node_31;
+  var inline$SpecGetRefVal$0$_heap: PolymorphicMapType_5887;
+  var inline$SpecGetRefVal$0$ref: Ref_5911;
+  var inline$SpecGetRefVal$0$x: Node_31;
+  var inline$SpecGetRefVal$0$heap: PolymorphicMapType_5887;
+  var inline$SpecGetRefVal$1$_heap: PolymorphicMapType_5887;
+  var inline$SpecGetRefVal$1$ref: Ref_5911;
+  var inline$SpecGetRefVal$1$x: Node_31;
+  var inline$SpecGetRefVal$1$heap: PolymorphicMapType_5887;
+  var inline$SpecSetRefVal$0$_heap: PolymorphicMapType_5887;
+  var inline$SpecSetRefVal$0$ref: Ref_5911;
+  var inline$SpecSetRefVal$0$x: Option_5934;
+  var inline$SpecSetRefVal$0$heap: PolymorphicMapType_5887;
+
+  /*** structured program:
+    call oldHead := SpecGetRefVal(head);
+    call newHead := SpecGetRefVal(oldHead->next);
+    call SpecSetRefVal(head, Some_5934(newHead));
+    item := oldHead->val;
+  **** end structured program */
+
+  anon0:
+    goto inline$SpecGetRefVal$0$Entry;
+
+  inline$SpecGetRefVal$0$Entry:
+    inline$SpecGetRefVal$0$ref := head;
+    havoc inline$SpecGetRefVal$0$_heap, inline$SpecGetRefVal$0$x;
+    inline$SpecGetRefVal$0$heap := heap;
+    goto inline$SpecGetRefVal$0$anon0;
+
+  inline$SpecGetRefVal$0$anon0:
+    inline$SpecGetRefVal$0$_heap := inline$SpecGetRefVal$0$heap;
+    inline$SpecGetRefVal$0$x := inline$SpecGetRefVal$0$_heap->PolymorphicMapType_5887_38[inline$SpecGetRefVal$0$ref]->t;
+    goto inline$SpecGetRefVal$0$Return;
+
+  inline$SpecGetRefVal$0$Return:
+    oldHead := inline$SpecGetRefVal$0$x;
+    goto anon0$1;
+
+  anon0$1:
+    goto inline$SpecGetRefVal$1$Entry;
+
+  inline$SpecGetRefVal$1$Entry:
+    inline$SpecGetRefVal$1$ref := oldHead->next;
+    havoc inline$SpecGetRefVal$1$_heap, inline$SpecGetRefVal$1$x;
+    inline$SpecGetRefVal$1$heap := heap;
+    goto inline$SpecGetRefVal$1$anon0;
+
+  inline$SpecGetRefVal$1$anon0:
+    inline$SpecGetRefVal$1$_heap := inline$SpecGetRefVal$1$heap;
+    inline$SpecGetRefVal$1$x := inline$SpecGetRefVal$1$_heap->PolymorphicMapType_5887_38[inline$SpecGetRefVal$1$ref]->t;
+    goto inline$SpecGetRefVal$1$Return;
+
+  inline$SpecGetRefVal$1$Return:
+    newHead := inline$SpecGetRefVal$1$x;
+    goto anon0$2;
+
+  anon0$2:
+    goto inline$SpecSetRefVal$0$Entry;
+
+  inline$SpecSetRefVal$0$Entry:
+    inline$SpecSetRefVal$0$ref := head;
+    inline$SpecSetRefVal$0$x := Some_5934(newHead);
+    havoc inline$SpecSetRefVal$0$_heap;
+    inline$SpecSetRefVal$0$heap := heap;
+    goto inline$SpecSetRefVal$0$anon0;
+
+  inline$SpecSetRefVal$0$anon0:
+    inline$SpecSetRefVal$0$_heap := inline$SpecSetRefVal$0$heap;
+    inline$SpecSetRefVal$0$_heap->PolymorphicMapType_5887_38[inline$SpecSetRefVal$0$ref] := inline$SpecSetRefVal$0$x;
+    goto inline$SpecSetRefVal$0$Return;
+
+  inline$SpecSetRefVal$0$Return:
+    goto anon0$3;
+
+  anon0$3:
+    item := oldHead->val;
+    return;
+}
+
+
+
+procedure {:inline 1} SpecPop() returns (item: int);
+  modifies heap, head;
+
+
+
+function {:inline} Civl_InputOutputRelation_SpecPop(item: int) : bool
+{
+  (exists Civl_old_heap: PolymorphicMapType_5887, 
+      Civl_old_head: Ref_5911, 
+      Civl_heap: PolymorphicMapType_5887, 
+      Civl_head: Ref_5911 :: 
+    item == Civl_heap->PolymorphicMapType_5887_38[Civl_head]->t->val
+       && Civl_heap == Civl_old_heap
+       && Civl_head == Civl_old_head)
 }
 
 implementation SpecPush(item: int)
 {
-  var newHeadRef: Lval_7085;
+  var newHeadRef: Lval_6847;
   var newHead: Node_31;
-  var inline$SpecAllocNodeRef$0$k: Lval_7085;
-  var inline$SpecAllocNodeRef$0$heap: PolymorphicMapType_5905;
-  var inline$SpecSetRefVal$0$_heap: PolymorphicMapType_5905;
-  var inline$SpecSetRefVal$0$ref: Ref_5929;
-  var inline$SpecSetRefVal$0$x: Option_5952;
-  var inline$SpecSetRefVal$0$heap: PolymorphicMapType_5905;
-  var inline$SpecGetRefVal$0$_heap: PolymorphicMapType_5905;
-  var inline$SpecGetRefVal$0$ref: Ref_5929;
+  var inline$SpecAllocNodeRef$0$k: Lval_6847;
+  var inline$SpecAllocNodeRef$0$heap: PolymorphicMapType_5887;
+  var inline$SpecSetRefVal$0$_heap: PolymorphicMapType_5887;
+  var inline$SpecSetRefVal$0$ref: Ref_5911;
+  var inline$SpecSetRefVal$0$x: Option_5934;
+  var inline$SpecSetRefVal$0$heap: PolymorphicMapType_5887;
+  var inline$SpecGetRefVal$0$_heap: PolymorphicMapType_5887;
+  var inline$SpecGetRefVal$0$ref: Ref_5911;
   var inline$SpecGetRefVal$0$x: Node_31;
-  var inline$SpecGetRefVal$0$heap: PolymorphicMapType_5905;
-  var inline$SpecSetRefVal$1$_heap: PolymorphicMapType_5905;
-  var inline$SpecSetRefVal$1$ref: Ref_5929;
-  var inline$SpecSetRefVal$1$x: Option_5952;
-  var inline$SpecSetRefVal$1$heap: PolymorphicMapType_5905;
+  var inline$SpecGetRefVal$0$heap: PolymorphicMapType_5887;
+  var inline$SpecSetRefVal$1$_heap: PolymorphicMapType_5887;
+  var inline$SpecSetRefVal$1$ref: Ref_5911;
+  var inline$SpecSetRefVal$1$x: Option_5934;
+  var inline$SpecSetRefVal$1$heap: PolymorphicMapType_5887;
 
   /*** structured program:
     call newHeadRef := SpecAllocNodeRef();
     call newHead := SpecGetRefVal(newHeadRef->val);
     newHead->next := head;
     newHead->val := item;
-    call SpecSetRefVal(head, Some_5952(newHead));
+    call SpecSetRefVal(head, Some_5934(newHead));
   **** end structured program */
 
   anon0:
@@ -519,19 +693,19 @@ implementation SpecPush(item: int)
   inline$SpecAllocNodeRef$0$anon0:
     havoc inline$SpecAllocNodeRef$0$k;
     assume Trigger_SpecPush_inline$SpecAllocNodeRef$0$k(inline$SpecAllocNodeRef$0$k);
-    assume inline$SpecAllocNodeRef$0$k->val != Nil_7109();
+    assume inline$SpecAllocNodeRef$0$k->val != Nil_6871();
     goto inline$SpecSetRefVal$0$Entry;
 
   inline$SpecSetRefVal$0$Entry:
     inline$SpecSetRefVal$0$ref := inline$SpecAllocNodeRef$0$k->val;
-    inline$SpecSetRefVal$0$x := None_5952();
+    inline$SpecSetRefVal$0$x := None_5934();
     havoc inline$SpecSetRefVal$0$_heap;
     inline$SpecSetRefVal$0$heap := heap;
     goto inline$SpecSetRefVal$0$anon0;
 
   inline$SpecSetRefVal$0$anon0:
     inline$SpecSetRefVal$0$_heap := inline$SpecSetRefVal$0$heap;
-    inline$SpecSetRefVal$0$_heap->PolymorphicMapType_5905_38[inline$SpecSetRefVal$0$ref] := inline$SpecSetRefVal$0$x;
+    inline$SpecSetRefVal$0$_heap->PolymorphicMapType_5887_38[inline$SpecSetRefVal$0$ref] := inline$SpecSetRefVal$0$x;
     goto inline$SpecSetRefVal$0$Return;
 
   inline$SpecSetRefVal$0$Return:
@@ -555,7 +729,7 @@ implementation SpecPush(item: int)
 
   inline$SpecGetRefVal$0$anon0:
     inline$SpecGetRefVal$0$_heap := inline$SpecGetRefVal$0$heap;
-    inline$SpecGetRefVal$0$x := inline$SpecGetRefVal$0$_heap->PolymorphicMapType_5905_38[inline$SpecGetRefVal$0$ref]->t;
+    inline$SpecGetRefVal$0$x := inline$SpecGetRefVal$0$_heap->PolymorphicMapType_5887_38[inline$SpecGetRefVal$0$ref]->t;
     goto inline$SpecGetRefVal$0$Return;
 
   inline$SpecGetRefVal$0$Return:
@@ -569,14 +743,14 @@ implementation SpecPush(item: int)
 
   inline$SpecSetRefVal$1$Entry:
     inline$SpecSetRefVal$1$ref := head;
-    inline$SpecSetRefVal$1$x := Some_5952(newHead);
+    inline$SpecSetRefVal$1$x := Some_5934(newHead);
     havoc inline$SpecSetRefVal$1$_heap;
     inline$SpecSetRefVal$1$heap := heap;
     goto inline$SpecSetRefVal$1$anon0;
 
   inline$SpecSetRefVal$1$anon0:
     inline$SpecSetRefVal$1$_heap := inline$SpecSetRefVal$1$heap;
-    inline$SpecSetRefVal$1$_heap->PolymorphicMapType_5905_38[inline$SpecSetRefVal$1$ref] := inline$SpecSetRefVal$1$x;
+    inline$SpecSetRefVal$1$_heap->PolymorphicMapType_5887_38[inline$SpecSetRefVal$1$ref] := inline$SpecSetRefVal$1$x;
     goto inline$SpecSetRefVal$1$Return;
 
   inline$SpecSetRefVal$1$Return:
@@ -595,12 +769,12 @@ procedure {:inline 1} SpecPush(item: int);
 
 function {:inline} Civl_InputOutputRelation_SpecPush(item: int) : bool
 {
-  (exists Civl_old_heap: PolymorphicMapType_5905, 
-      Civl_old_head: Ref_5929, 
-      Civl_heap: PolymorphicMapType_5905, 
-      Civl_head: Ref_5929, 
-      Civl_inline$SpecAllocNodeRef$0$k#2: Lval_7085 :: 
-    Civl_inline$SpecAllocNodeRef$0$k#2->val != Nil_7109()
+  (exists Civl_old_heap: PolymorphicMapType_5887, 
+      Civl_old_head: Ref_5911, 
+      Civl_heap: PolymorphicMapType_5887, 
+      Civl_head: Ref_5911, 
+      Civl_inline$SpecAllocNodeRef$0$k#2: Lval_6847 :: 
+    Civl_inline$SpecAllocNodeRef$0$k#2->val != Nil_6871()
        && Civl_heap == Civl_old_heap)
 }
 
@@ -619,19 +793,19 @@ procedure {:inline 1} Civl_Skip();
 
 function {:inline} Civl_InputOutputRelation_Civl_Skip() : bool
 {
-  (exists Civl_old_heap: PolymorphicMapType_5905, 
-      Civl_old_head: Ref_5929, 
-      Civl_heap: PolymorphicMapType_5905, 
-      Civl_head: Ref_5929 :: 
+  (exists Civl_old_heap: PolymorphicMapType_5887, 
+      Civl_old_head: Ref_5911, 
+      Civl_heap: PolymorphicMapType_5887, 
+      Civl_head: Ref_5911 :: 
     true)
 }
 
-procedure Civl_SetRefVal_0(ref: Ref_5929, x: Option_5952);
+procedure Civl_SetRefVal_0(ref: Ref_5911, x: Option_5934);
   modifies heap, head;
 
 
 
-procedure Civl_GetRefVal_0(ref: Ref_5929) returns (x: Node_31);
+procedure Civl_GetRefVal_0(ref: Ref_5911) returns (x: Node_31);
   modifies heap, head;
 
 
@@ -646,7 +820,7 @@ procedure Civl_CAS_Head_0(expectedNode: Node_31, desiredNode: Node_31) returns (
 
 
 
-procedure Civl_AllocNodeRef_0() returns (k: Lval_7085);
+procedure Civl_AllocNodeRef_0() returns (k: Lval_6847);
   modifies heap, head;
 
 
@@ -663,13 +837,13 @@ procedure Civl_Push_0(item: int);
 
 implementation Civl_NodeEq_0(n1: Node_31, n2: Node_31) returns (eq: bool)
 {
-  var Civl_global_old_heap: PolymorphicMapType_5905;
-  var Civl_global_old_head: Ref_5929;
+  var Civl_global_old_heap: PolymorphicMapType_5887;
+  var Civl_global_old_head: Ref_5911;
   var Civl_pc: bool;
   var Civl_ok: bool;
   var Civl_eval: bool;
   var Civl_old_eq: bool;
-  var Civl_linear_Ref_5929_available: [Ref_5929]bool;
+  var Civl_linear_Ref_5911_available: [Ref_5911]bool;
 
   /*** structured program:
     eq := n1->val == n2->val && n1->next == n2->next;
@@ -681,7 +855,7 @@ implementation Civl_NodeEq_0(n1: Node_31, n2: Node_31) returns (eq: bool)
     Civl_pc, Civl_ok, Civl_eval := false, false, false;
     Civl_old_eq := eq;
     assume true;
-    Civl_linear_Ref_5929_available := MapConst_5_7085(false);
+    Civl_linear_Ref_5911_available := MapConst_5_6847(false);
     goto anon0;
 
   anon0:
@@ -689,7 +863,7 @@ implementation Civl_NodeEq_0(n1: Node_31, n2: Node_31) returns (eq: bool)
     goto Civl_ReturnChecker, Civl_UnifiedReturn, Civl_NoninterferenceChecker;
 
   Civl_NoninterferenceChecker:
-    call Civl_Wrapper_NoninterferenceChecker_0(Civl_linear_Ref_5929_available, Civl_global_old_heap, Civl_global_old_head);
+    call Civl_Wrapper_NoninterferenceChecker_0(Civl_linear_Ref_5911_available, Civl_global_old_heap, Civl_global_old_head);
     assume false;
     return;
 
@@ -734,206 +908,28 @@ implementation Civl_NodeEq_0(n1: Node_31, n2: Node_31) returns (eq: bool)
 
 
 
-implementation Civl_CAS_Head_0(expectedNode: Node_31, desiredNode: Node_31) returns (success: bool)
-{
-  var eq: bool;
-  var headNode: Node_31;
-  var _head: Ref_5929;
-  var _heap: PolymorphicMapType_5905;
-  var Civl_global_old_heap: PolymorphicMapType_5905;
-  var Civl_global_old_head: Ref_5929;
-  var Civl_pc: bool;
-  var Civl_ok: bool;
-  var Civl_eval: bool;
-  var Civl_old_success: bool;
-  var Civl_linear_Ref_5929_available: [Ref_5929]bool;
-
-  /*** structured program:
-    _head := old(head);
-    call headNode := GetRefVal(_head);
-    call eq := NodeEq(headNode, expectedNode);
-    if (eq)
-    {
-        call SetRefVal(_head, Some_5952(desiredNode));
-        success := true;
-    }
-    else
-    {
-        success := false;
-    }
-  **** end structured program */
-
-  Civl_init:
-    havoc heap, head;
-    Civl_global_old_heap, Civl_global_old_head := heap, head;
-    Civl_pc, Civl_ok, Civl_eval := false, false, false;
-    Civl_old_success := success;
-    assume true;
-    Civl_linear_Ref_5929_available := MapConst_5_7085(false);
-    goto anon0;
-
-  anon0:
-    _head := old(head);
-    Civl_eval := (
-        heap->PolymorphicMapType_5905_38[head]->t == expectedNode
-         && heap == Civl_global_old_heap
-         && head == Civl_global_old_head)
-       || (
-        !(heap->PolymorphicMapType_5905_38[head]->t == expectedNode)
-         && heap == Civl_global_old_heap
-         && head == Civl_global_old_head);
-    goto anon0_1, Civl_call_refinement_0, Civl_NoninterferenceChecker, Civl_RefinementChecker;
-
-  anon0_1:
-    Civl_pc, Civl_ok := heap == Civl_global_old_heap && head == Civl_global_old_head ==> Civl_pc, Civl_eval || ((success <==> Civl_old_success) && Civl_ok);
-    call headNode := Civl_ParallelCall_GetRefVal_0(_head);
-    assume Civl_pc || true;
-    Civl_global_old_heap, Civl_global_old_head := heap, head;
-    Civl_old_success := success;
-    Civl_linear_Ref_5929_available := MapConst_5_7085(false);
-    Civl_eval := (
-        heap->PolymorphicMapType_5905_38[head]->t == expectedNode
-         && heap == Civl_global_old_heap
-         && head == Civl_global_old_head)
-       || (
-        !(heap->PolymorphicMapType_5905_38[head]->t == expectedNode)
-         && heap == Civl_global_old_heap
-         && head == Civl_global_old_head);
-    goto anon0_0, Civl_call_refinement_1, Civl_NoninterferenceChecker, Civl_RefinementChecker;
-
-  anon0_0:
-    Civl_pc, Civl_ok := heap == Civl_global_old_heap && head == Civl_global_old_head ==> Civl_pc, Civl_eval || ((success <==> Civl_old_success) && Civl_ok);
-    call eq := Civl_ParallelCall_NodeEq_0(headNode, expectedNode);
-    assume Civl_pc || true;
-    Civl_global_old_heap, Civl_global_old_head := heap, head;
-    Civl_old_success := success;
-    Civl_linear_Ref_5929_available := MapConst_5_7085(false);
-    goto anon3_Then, anon3_Else;
-
-  anon3_Else:
-    assume {:partition} !eq;
-    success := false;
-    goto Civl_ReturnChecker, Civl_UnifiedReturn, Civl_NoninterferenceChecker;
-
-  anon3_Then:
-    assume {:partition} eq;
-    Civl_eval := (
-        heap->PolymorphicMapType_5905_38[head]->t == expectedNode
-         && heap == Civl_global_old_heap
-         && head == Civl_global_old_head)
-       || (
-        !(heap->PolymorphicMapType_5905_38[head]->t == expectedNode)
-         && heap == Civl_global_old_heap
-         && head == Civl_global_old_head);
-    goto anon3_Then_0, Civl_call_refinement_2, Civl_NoninterferenceChecker, Civl_RefinementChecker;
-
-  anon3_Then_0:
-    Civl_pc, Civl_ok := heap == Civl_global_old_heap && head == Civl_global_old_head ==> Civl_pc, Civl_eval || ((success <==> Civl_old_success) && Civl_ok);
-    call Civl_ParallelCall_SetRefVal_0(_head, Some_5952(desiredNode));
-    assume Civl_pc || true;
-    Civl_global_old_heap, Civl_global_old_head := heap, head;
-    Civl_old_success := success;
-    Civl_linear_Ref_5929_available := MapConst_5_7085(false);
-    success := true;
-    goto Civl_ReturnChecker, Civl_UnifiedReturn, Civl_NoninterferenceChecker;
-
-  Civl_NoninterferenceChecker:
-    call Civl_Wrapper_NoninterferenceChecker_0(Civl_linear_Ref_5929_available, Civl_global_old_heap, Civl_global_old_head);
-    assume false;
-    return;
-
-  Civl_RefinementChecker:
-    assert Civl_pc
-       || 
-      (heap == Civl_global_old_heap && head == Civl_global_old_head)
-       || Civl_eval;
-    assert Civl_pc
-       ==> heap == Civl_global_old_heap
-         && head == Civl_global_old_head
-         && (success <==> Civl_old_success);
-    assume false;
-    return;
-
-  Civl_UnchangedChecker:
-    assert heap == Civl_global_old_heap && head == Civl_global_old_head;
-    assert Civl_pc ==> (success <==> Civl_old_success);
-    assume false;
-    return;
-
-  Civl_ReturnChecker:
-    Civl_eval := (
-        heap->PolymorphicMapType_5905_38[head]->t == expectedNode
-         && heap == Civl_global_old_heap
-         && head == Civl_global_old_head)
-       || (
-        !(heap->PolymorphicMapType_5905_38[head]->t == expectedNode)
-         && heap == Civl_global_old_heap
-         && head == Civl_global_old_head);
-    assert Civl_pc
-       || 
-      (heap == Civl_global_old_heap && head == Civl_global_old_head)
-       || Civl_eval;
-    assert Civl_pc
-       ==> heap == Civl_global_old_heap
-         && head == Civl_global_old_head
-         && (success <==> Civl_old_success);
-    Civl_pc, Civl_ok := heap == Civl_global_old_heap && head == Civl_global_old_head ==> Civl_pc, Civl_eval || ((success <==> Civl_old_success) && Civl_ok);
-    assert Civl_ok;
-    assume false;
-    return;
-
-  Civl_UnifiedReturn:
-    return;
-
-  Civl_call_refinement_0:
-    havoc heap, head;
-    assume Civl_pc || true;
-    Civl_global_old_heap, Civl_global_old_head := heap, head;
-    Civl_old_success := success;
-    call headNode := SpecGetRefVal(_head);
-    goto Civl_UnchangedChecker;
-
-  Civl_call_refinement_1:
-    havoc heap, head;
-    assume Civl_pc || true;
-    Civl_global_old_heap, Civl_global_old_head := heap, head;
-    Civl_old_success := success;
-    call eq := SpecNodeEq(headNode, expectedNode);
-    goto Civl_UnchangedChecker;
-
-  Civl_call_refinement_2:
-    havoc heap, head;
-    assume Civl_pc || true;
-    Civl_global_old_heap, Civl_global_old_head := heap, head;
-    Civl_old_success := success;
-    call SpecSetRefVal(_head, Some_5952(desiredNode));
-    goto Civl_UnchangedChecker;
-}
-
-
-
 implementation Civl_Pop_0() returns (item: int)
 {
   var oldHead: Node_31;
   var newHead: Node_31;
   var cas_success: bool;
-  var Civl_global_old_heap: PolymorphicMapType_5905;
-  var Civl_global_old_head: Ref_5929;
-  var Civl_linear_Ref_5929_available: [Ref_5929]bool;
+  var Civl_global_old_heap: PolymorphicMapType_5887;
+  var Civl_global_old_head: Ref_5911;
+  var Civl_linear_Ref_5911_available: [Ref_5911]bool;
 
   /*** structured program:
     while (true)
       invariant {:yields} true;
     {
-        oldHead := old(heap->PolymorphicMapType_5905_38[head]->t);
-        newHead := old(heap->PolymorphicMapType_5905_38[oldHead->next]->t);
+        oldHead := old(heap->PolymorphicMapType_5887_38[head]->t);
+        newHead := old(heap->PolymorphicMapType_5887_38[oldHead->next]->t);
         call cas_success := CAS_Head(oldHead, newHead);
         if (cas_success)
         {
             item := oldHead->val;
-            assert item == old(heap->PolymorphicMapType_5905_38[head]->t->val);
+            assert item == old(heap->PolymorphicMapType_5887_38[head]->t->val);
             assert newHead
-               == old(heap->PolymorphicMapType_5905_38[heap->PolymorphicMapType_5905_38[head]->t->next]->t);
+               == old(heap->PolymorphicMapType_5887_38[heap->PolymorphicMapType_5887_38[head]->t->next]->t);
             break;
         }
     }
@@ -942,7 +938,7 @@ implementation Civl_Pop_0() returns (item: int)
   Civl_init:
     havoc heap, head;
     Civl_global_old_heap, Civl_global_old_head := heap, head;
-    Civl_linear_Ref_5929_available := MapConst_5_7085(false);
+    Civl_linear_Ref_5911_available := MapConst_5_6847(false);
     goto anon0;
 
   anon0:
@@ -951,19 +947,19 @@ implementation Civl_Pop_0() returns (item: int)
   anon3_LoopHead:
     heap, head := heap, head;
     Civl_global_old_heap, Civl_global_old_head := heap, head;
-    Civl_linear_Ref_5929_available := MapConst_5_7085(false);
+    Civl_linear_Ref_5911_available := MapConst_5_6847(false);
     goto anon3_LoopDone, anon3_LoopBody;
 
   anon3_LoopBody:
     assume {:partition} true;
-    oldHead := old(heap->PolymorphicMapType_5905_38[head]->t);
-    newHead := old(heap->PolymorphicMapType_5905_38[oldHead->next]->t);
+    oldHead := old(heap->PolymorphicMapType_5887_38[head]->t);
+    newHead := old(heap->PolymorphicMapType_5887_38[oldHead->next]->t);
     goto anon3_LoopBody_0, Civl_NoninterferenceChecker, Civl_UnchangedChecker;
 
   anon3_LoopBody_0:
     call cas_success := Civl_ParallelCall_CAS_Head_0(oldHead, newHead);
     Civl_global_old_heap, Civl_global_old_head := heap, head;
-    Civl_linear_Ref_5929_available := MapConst_5_7085(false);
+    Civl_linear_Ref_5911_available := MapConst_5_6847(false);
     goto anon4_Then, anon4_Else;
 
   anon4_Else:
@@ -982,7 +978,7 @@ implementation Civl_Pop_0() returns (item: int)
     goto Civl_ReturnChecker, Civl_UnifiedReturn, Civl_NoninterferenceChecker;
 
   Civl_NoninterferenceChecker:
-    call Civl_Wrapper_NoninterferenceChecker_0(Civl_linear_Ref_5929_available, Civl_global_old_heap, Civl_global_old_head);
+    call Civl_Wrapper_NoninterferenceChecker_0(Civl_linear_Ref_5911_available, Civl_global_old_heap, Civl_global_old_head);
     assume false;
     return;
 
@@ -1006,25 +1002,25 @@ implementation Civl_Pop_0() returns (item: int)
 
 implementation Civl_Push_0(item: int)
 {
-  var oldHeadRef: Ref_5929;
+  var oldHeadRef: Ref_5911;
   var oldHead: Node_31;
-  var newHeadRef: Lval_7085;
+  var newHeadRef: Lval_6847;
   var newHead: Node_31;
   var cas_success: bool;
-  var Civl_global_old_heap: PolymorphicMapType_5905;
-  var Civl_global_old_head: Ref_5929;
-  var Civl_linear_Ref_5929_available: [Ref_5929]bool;
+  var Civl_global_old_heap: PolymorphicMapType_5887;
+  var Civl_global_old_head: Ref_5911;
+  var Civl_linear_Ref_5911_available: [Ref_5911]bool;
 
   /*** structured program:
     call newHeadRef := AllocNodeRef();
-    newHead := old(heap->PolymorphicMapType_5905_38[newHeadRef->val]->t);
+    newHead := old(heap->PolymorphicMapType_5887_38[newHeadRef->val]->t);
     newHead->val := item;
     while (true)
       invariant {:yields} true;
     {
         oldHeadRef := old(head);
         newHead->next := oldHeadRef;
-        oldHead := old(heap->PolymorphicMapType_5905_38[newHead->next]->t);
+        oldHead := old(heap->PolymorphicMapType_5887_38[newHead->next]->t);
         call cas_success := CAS_Head(oldHead, newHead);
         if (cas_success)
         {
@@ -1037,7 +1033,7 @@ implementation Civl_Push_0(item: int)
   Civl_init:
     havoc heap, head;
     Civl_global_old_heap, Civl_global_old_head := heap, head;
-    Civl_linear_Ref_5929_available := MapConst_5_7085(false);
+    Civl_linear_Ref_5911_available := MapConst_5_6847(false);
     goto anon0;
 
   anon0:
@@ -1046,28 +1042,28 @@ implementation Civl_Push_0(item: int)
   anon0_0:
     call newHeadRef := Civl_ParallelCall_AllocNodeRef_0();
     Civl_global_old_heap, Civl_global_old_head := heap, head;
-    Civl_linear_Ref_5929_available := MapOr_7085(Lval_Collector_7085(newHeadRef), MapConst_5_7085(false));
-    newHead := old(heap->PolymorphicMapType_5905_38[newHeadRef->val]->t);
+    Civl_linear_Ref_5911_available := MapOr_6847(Lval_Collector_6847(newHeadRef), MapConst_5_6847(false));
+    newHead := old(heap->PolymorphicMapType_5887_38[newHeadRef->val]->t);
     newHead->val := item;
     goto anon3_LoopHead, Civl_NoninterferenceChecker, Civl_RefinementChecker;
 
   anon3_LoopHead:
     heap, head := heap, head;
     Civl_global_old_heap, Civl_global_old_head := heap, head;
-    Civl_linear_Ref_5929_available := MapOr_7085(Lval_Collector_7085(newHeadRef), MapConst_5_7085(false));
+    Civl_linear_Ref_5911_available := MapOr_6847(Lval_Collector_6847(newHeadRef), MapConst_5_6847(false));
     goto anon3_LoopDone, anon3_LoopBody;
 
   anon3_LoopBody:
     assume {:partition} true;
     oldHeadRef := old(head);
     newHead->next := oldHeadRef;
-    oldHead := old(heap->PolymorphicMapType_5905_38[newHead->next]->t);
+    oldHead := old(heap->PolymorphicMapType_5887_38[newHead->next]->t);
     goto anon3_LoopBody_0, Civl_NoninterferenceChecker, Civl_UnchangedChecker;
 
   anon3_LoopBody_0:
     call cas_success := Civl_ParallelCall_CAS_Head_0(oldHead, newHead);
     Civl_global_old_heap, Civl_global_old_head := heap, head;
-    Civl_linear_Ref_5929_available := MapOr_7085(Lval_Collector_7085(newHeadRef), MapConst_5_7085(false));
+    Civl_linear_Ref_5911_available := MapOr_6847(Lval_Collector_6847(newHeadRef), MapConst_5_6847(false));
     goto anon4_Then, anon4_Else;
 
   anon4_Else:
@@ -1084,7 +1080,7 @@ implementation Civl_Push_0(item: int)
     goto Civl_ReturnChecker, Civl_UnifiedReturn, Civl_NoninterferenceChecker;
 
   Civl_NoninterferenceChecker:
-    call Civl_Wrapper_NoninterferenceChecker_0(Civl_linear_Ref_5929_available, Civl_global_old_heap, Civl_global_old_head);
+    call Civl_Wrapper_NoninterferenceChecker_0(Civl_linear_Ref_5911_available, Civl_global_old_heap, Civl_global_old_head);
     assume false;
     return;
 
@@ -1106,41 +1102,26 @@ implementation Civl_Push_0(item: int)
 
 
 
-procedure Civl_ParallelCall_GetRefVal_0(Civl_0_ref: Ref_5929) returns (Civl_0_x: Node_31);
-  modifies heap, head;
-
-
-
-procedure Civl_ParallelCall_NodeEq_0(Civl_0_n1: Node_31, Civl_0_n2: Node_31) returns (Civl_0_eq: bool);
-  modifies heap, head;
-
-
-
-procedure Civl_ParallelCall_SetRefVal_0(Civl_0_ref: Ref_5929, Civl_0_x: Option_5952);
-  modifies heap, head;
-
-
-
 procedure Civl_ParallelCall_CAS_Head_0(Civl_0_expectedNode: Node_31, Civl_0_desiredNode: Node_31)
    returns (Civl_0_success: bool);
   modifies heap, head;
 
 
 
-procedure Civl_ParallelCall_AllocNodeRef_0() returns (Civl_0_k: Lval_7085);
+procedure Civl_ParallelCall_AllocNodeRef_0() returns (Civl_0_k: Lval_6847);
   modifies heap, head;
 
 
 
-procedure {:inline 1} Civl_Wrapper_NoninterferenceChecker_0(Civl_linear_Ref_5929_in: [Ref_5929]bool, 
-    Civl_global_old_heap: PolymorphicMapType_5905, 
-    Civl_global_old_head: Ref_5929);
+procedure {:inline 1} Civl_Wrapper_NoninterferenceChecker_0(Civl_linear_Ref_5911_in: [Ref_5911]bool, 
+    Civl_global_old_heap: PolymorphicMapType_5887, 
+    Civl_global_old_head: Ref_5911);
 
 
 
-implementation Civl_Wrapper_NoninterferenceChecker_0(Civl_Civl_linear_Ref_5929_in: [Ref_5929]bool, 
-    Civl_Civl_global_old_heap: PolymorphicMapType_5905, 
-    Civl_Civl_global_old_head: Ref_5929)
+implementation Civl_Wrapper_NoninterferenceChecker_0(Civl_Civl_linear_Ref_5911_in: [Ref_5911]bool, 
+    Civl_Civl_global_old_heap: PolymorphicMapType_5887, 
+    Civl_Civl_global_old_head: Ref_5911)
 {
 
   enter:
@@ -1150,7 +1131,7 @@ implementation Civl_Wrapper_NoninterferenceChecker_0(Civl_Civl_linear_Ref_5929_i
 
 
 procedure Civl_Pop_1() returns (item: int);
-  modifies heap;
+  modifies heap, head;
 
 
 
@@ -1164,52 +1145,116 @@ implementation Civl_Pop_1() returns (item: int)
   var oldHead: Node_31;
   var newHead: Node_31;
   var cas_success: bool;
+  var Civl_global_old_heap: PolymorphicMapType_5887;
+  var Civl_global_old_head: Ref_5911;
+  var Civl_pc: bool;
+  var Civl_ok: bool;
+  var Civl_eval: bool;
+  var Civl_old_item: int;
+  var Civl_linear_Ref_5911_available: [Ref_5911]bool;
 
   /*** structured program:
     while (true)
       invariant {:yields} true;
     {
-        oldHead := old(heap->PolymorphicMapType_5905_38[head]->t);
-        newHead := old(heap->PolymorphicMapType_5905_38[oldHead->next]->t);
+        oldHead := old(heap->PolymorphicMapType_5887_38[head]->t);
+        newHead := old(heap->PolymorphicMapType_5887_38[oldHead->next]->t);
         call cas_success := CAS_Head(oldHead, newHead);
         if (cas_success)
         {
             item := oldHead->val;
-            assert item == old(heap->PolymorphicMapType_5905_38[head]->t->val);
+            assert item == old(heap->PolymorphicMapType_5887_38[head]->t->val);
             assert newHead
-               == old(heap->PolymorphicMapType_5905_38[heap->PolymorphicMapType_5905_38[head]->t->next]->t);
+               == old(heap->PolymorphicMapType_5887_38[heap->PolymorphicMapType_5887_38[head]->t->next]->t);
             break;
         }
     }
   **** end structured program */
 
+  Civl_init:
+    havoc heap, head;
+    Civl_global_old_heap, Civl_global_old_head := heap, head;
+    Civl_pc, Civl_ok, Civl_eval := false, false, false;
+    Civl_old_item := item;
+    assume true;
+    Civl_linear_Ref_5911_available := MapConst_5_6847(false);
+    goto anon0;
+
   anon0:
-    goto anon3_LoopHead;
+    goto anon3_LoopHead, Civl_NoninterferenceChecker, Civl_RefinementChecker;
 
   anon3_LoopHead:
+    assume Civl_pc || true;
+    heap, head := heap, head;
+    Civl_global_old_heap, Civl_global_old_head := heap, head;
+    Civl_old_item := item;
+    Civl_linear_Ref_5911_available := MapConst_5_6847(false);
     goto anon3_LoopDone, anon3_LoopBody;
 
   anon3_LoopBody:
     assume {:partition} true;
-    oldHead := old(heap->PolymorphicMapType_5905_38[head]->t);
-    newHead := old(heap->PolymorphicMapType_5905_38[oldHead->next]->t);
+    oldHead := old(heap->PolymorphicMapType_5887_38[head]->t);
+    newHead := old(heap->PolymorphicMapType_5887_38[oldHead->next]->t);
     call cas_success := SpecCAS_Head(oldHead, newHead);
     goto anon4_Then, anon4_Else;
 
   anon4_Else:
     assume {:partition} !cas_success;
-    goto anon3_LoopHead;
+    goto anon3_LoopHead, Civl_NoninterferenceChecker, Civl_UnchangedChecker;
 
   anon4_Then:
     assume {:partition} cas_success;
     item := oldHead->val;
-    assert item == old(heap->PolymorphicMapType_5905_38[head]->t->val);
+    assert item == old(heap->PolymorphicMapType_5887_38[head]->t->val);
     assert newHead
-       == old(heap->PolymorphicMapType_5905_38[heap->PolymorphicMapType_5905_38[head]->t->next]->t);
-    return;
+       == old(heap->PolymorphicMapType_5887_38[heap->PolymorphicMapType_5887_38[head]->t->next]->t);
+    goto Civl_ReturnChecker, Civl_UnifiedReturn, Civl_NoninterferenceChecker;
 
   anon3_LoopDone:
     assume {:partition} !true;
+    goto Civl_ReturnChecker, Civl_UnifiedReturn, Civl_NoninterferenceChecker;
+
+  Civl_NoninterferenceChecker:
+    call Civl_Wrapper_NoninterferenceChecker_1(Civl_linear_Ref_5911_available, Civl_global_old_heap, Civl_global_old_head);
+    assume false;
+    return;
+
+  Civl_RefinementChecker:
+    assert Civl_pc
+       || 
+      (heap == Civl_global_old_heap && head == Civl_global_old_head)
+       || Civl_eval;
+    assert Civl_pc
+       ==> heap == Civl_global_old_heap
+         && head == Civl_global_old_head
+         && item == Civl_old_item;
+    assume false;
+    return;
+
+  Civl_UnchangedChecker:
+    assert heap == Civl_global_old_heap && head == Civl_global_old_head;
+    assert Civl_pc ==> item == Civl_old_item;
+    assume false;
+    return;
+
+  Civl_ReturnChecker:
+    Civl_eval := item == heap->PolymorphicMapType_5887_38[head]->t->val
+       && heap == Civl_global_old_heap
+       && head == Civl_global_old_head;
+    assert Civl_pc
+       || 
+      (heap == Civl_global_old_heap && head == Civl_global_old_head)
+       || Civl_eval;
+    assert Civl_pc
+       ==> heap == Civl_global_old_heap
+         && head == Civl_global_old_head
+         && item == Civl_old_item;
+    Civl_pc, Civl_ok := heap == Civl_global_old_heap && head == Civl_global_old_head ==> Civl_pc, Civl_eval || (item == Civl_old_item && Civl_ok);
+    assert Civl_ok;
+    assume false;
+    return;
+
+  Civl_UnifiedReturn:
     return;
 }
 
@@ -1217,28 +1262,28 @@ implementation Civl_Pop_1() returns (item: int)
 
 implementation Civl_Push_1(item: int)
 {
-  var oldHeadRef: Ref_5929;
+  var oldHeadRef: Ref_5911;
   var oldHead: Node_31;
-  var newHeadRef: Lval_7085;
+  var newHeadRef: Lval_6847;
   var newHead: Node_31;
   var cas_success: bool;
-  var Civl_global_old_heap: PolymorphicMapType_5905;
-  var Civl_global_old_head: Ref_5929;
+  var Civl_global_old_heap: PolymorphicMapType_5887;
+  var Civl_global_old_head: Ref_5911;
   var Civl_pc: bool;
   var Civl_ok: bool;
   var Civl_eval: bool;
-  var Civl_linear_Ref_5929_available: [Ref_5929]bool;
+  var Civl_linear_Ref_5911_available: [Ref_5911]bool;
 
   /*** structured program:
     call newHeadRef := AllocNodeRef();
-    newHead := old(heap->PolymorphicMapType_5905_38[newHeadRef->val]->t);
+    newHead := old(heap->PolymorphicMapType_5887_38[newHeadRef->val]->t);
     newHead->val := item;
     while (true)
       invariant {:yields} true;
     {
         oldHeadRef := old(head);
         newHead->next := oldHeadRef;
-        oldHead := old(heap->PolymorphicMapType_5905_38[newHead->next]->t);
+        oldHead := old(heap->PolymorphicMapType_5887_38[newHead->next]->t);
         call cas_success := CAS_Head(oldHead, newHead);
         if (cas_success)
         {
@@ -1253,12 +1298,12 @@ implementation Civl_Push_1(item: int)
     Civl_global_old_heap, Civl_global_old_head := heap, head;
     Civl_pc, Civl_ok, Civl_eval := false, false, false;
     assume true;
-    Civl_linear_Ref_5929_available := MapConst_5_7085(false);
+    Civl_linear_Ref_5911_available := MapConst_5_6847(false);
     goto anon0;
 
   anon0:
     call newHeadRef := SpecAllocNodeRef();
-    newHead := old(heap->PolymorphicMapType_5905_38[newHeadRef->val]->t);
+    newHead := old(heap->PolymorphicMapType_5887_38[newHeadRef->val]->t);
     newHead->val := item;
     goto anon3_LoopHead, Civl_NoninterferenceChecker, Civl_RefinementChecker;
 
@@ -1266,14 +1311,14 @@ implementation Civl_Push_1(item: int)
     assume Civl_pc || true;
     heap, head := heap, head;
     Civl_global_old_heap, Civl_global_old_head := heap, head;
-    Civl_linear_Ref_5929_available := MapOr_7085(Lval_Collector_7085(newHeadRef), MapConst_5_7085(false));
+    Civl_linear_Ref_5911_available := MapOr_6847(Lval_Collector_6847(newHeadRef), MapConst_5_6847(false));
     goto anon3_LoopDone, anon3_LoopBody;
 
   anon3_LoopBody:
     assume {:partition} true;
     oldHeadRef := old(head);
     newHead->next := oldHeadRef;
-    oldHead := old(heap->PolymorphicMapType_5905_38[newHead->next]->t);
+    oldHead := old(heap->PolymorphicMapType_5887_38[newHead->next]->t);
     call cas_success := SpecCAS_Head(oldHead, newHead);
     goto anon4_Then, anon4_Else;
 
@@ -1291,7 +1336,7 @@ implementation Civl_Push_1(item: int)
     goto Civl_ReturnChecker, Civl_UnifiedReturn, Civl_NoninterferenceChecker;
 
   Civl_NoninterferenceChecker:
-    call Civl_Wrapper_NoninterferenceChecker_1(Civl_linear_Ref_5929_available, Civl_global_old_heap, Civl_global_old_head);
+    call Civl_Wrapper_NoninterferenceChecker_1(Civl_linear_Ref_5911_available, Civl_global_old_heap, Civl_global_old_head);
     assume false;
     return;
 
@@ -1311,8 +1356,8 @@ implementation Civl_Push_1(item: int)
     return;
 
   Civl_ReturnChecker:
-    Civl_eval := (exists Civl_inline$SpecAllocNodeRef$0$k#2: Lval_7085 :: 
-      Civl_inline$SpecAllocNodeRef$0$k#2->val != Nil_7109()
+    Civl_eval := (exists Civl_inline$SpecAllocNodeRef$0$k#2: Lval_6847 :: 
+      Civl_inline$SpecAllocNodeRef$0$k#2->val != Nil_6871()
          && heap == Civl_global_old_heap
          && head == Civl_global_old_head);
     assert Civl_pc
@@ -1331,15 +1376,15 @@ implementation Civl_Push_1(item: int)
 
 
 
-procedure {:inline 1} Civl_Wrapper_NoninterferenceChecker_1(Civl_linear_Ref_5929_in: [Ref_5929]bool, 
-    Civl_global_old_heap: PolymorphicMapType_5905, 
-    Civl_global_old_head: Ref_5929);
+procedure {:inline 1} Civl_Wrapper_NoninterferenceChecker_1(Civl_linear_Ref_5911_in: [Ref_5911]bool, 
+    Civl_global_old_heap: PolymorphicMapType_5887, 
+    Civl_global_old_head: Ref_5911);
 
 
 
-implementation Civl_Wrapper_NoninterferenceChecker_1(Civl_Civl_linear_Ref_5929_in: [Ref_5929]bool, 
-    Civl_Civl_global_old_heap: PolymorphicMapType_5905, 
-    Civl_Civl_global_old_head: Ref_5929)
+implementation Civl_Wrapper_NoninterferenceChecker_1(Civl_Civl_linear_Ref_5911_in: [Ref_5911]bool, 
+    Civl_Civl_global_old_heap: PolymorphicMapType_5887, 
+    Civl_Civl_global_old_head: Ref_5911)
 {
 
   enter:
